Attempt at relations for enc-enc integ spec.

verified/sec_prop.s.dfy
@@ -87,8 +87,13 @@ predicate enc_enc_conf_eq(s1:state, s2:state, d1:PageDb, d2:PageDb,
     configs_usr_equiv(s1, s2) &&
     nonStoppedL1(d1, l1p) <==> nonStoppedL1(d2, l1p) &&
     nonStoppedL1(d1, l1p) ==>
+        (var atkr_pgs := PagesInTable(mkAbsPTable(d1, l1p));
+        // The set of pages the enclave can observe is the same
         (PagesInTable(mkAbsPTable(d1, l1p)) == 
-            PagesInTable(mkAbsPTable(d2, l1p)))
+            PagesInTable(mkAbsPTable(d2, l1p))) &&
+        // The contents of those addresses is the same
+        (forall a | a in TheValidAddresses() && a in atkr_pgs ::
+            s1.m.addresses[a] == s2.m.addresses[a]))
 
 }
 
@@ -129,10 +134,58 @@ predicate configs_usr_equiv(s1:state, s2: state)
 
 function PagesInTable(pt:AbsPTable): set<addr>
     requires WellformedAbsPTable(pt)
-    ensures forall m:addr :: m in WritablePagesInTable(pt) ==> PageAligned(m)
+    ensures forall m:addr :: m in PagesInTable(pt) ==> PageAligned(m)
 {
     (set i, j | 0 <= i < |pt| && pt[i].Just? && 0 <= j < |pt[i].v|
         && pt[i].v[j].Just?
         :: (assert WellformedAbsPTE(pt[i].v[j]);
           pt[i].v[j].v.phys + PhysBase()))
+}
+
+//-----------------------------------------------------------------------------
+// Enclave-Enclave Integrity
+//-----------------------------------------------------------------------------
+// These relate states if the parts that the attacker cannot modify are the 
+// same in both.
+predicate enc_enc_integ_eqpdb(d1:PageDb, d2: PageDb, atkr:PageNr)
+    requires validPageDb(d1) && validPageDb(d2)
+    requires valDispPage(d1, atkr)
+{
+    var atkr_asp := d1[atkr].addrspace;
+    // The dispPage & addrspace are the same in both states.
+    valDispPage(d2, atkr) &&
+    d1[atkr].addrspace == d2[atkr].addrspace &&
+    valAddrPage(d1, atkr_asp) && valAddrPage(d2, atkr_asp) &&
+    (forall n : PageNr :: pgInAddrSpc(d1, n, atkr_asp) <==>
+        pgInAddrSpc(d2, n, atkr_asp)) &&
+    // The pages outside of the attacker's address space are the same
+    (forall n : PageNr | !pgInAddrSpc(d1, n, atkr_asp) :: 
+        d1[n].PageDbEntryTyped? <==> d2[n].PageDbEntryTyped?) &&
+    (forall n : PageNr | !pgInAddrSpc(d1, n, atkr_asp) && 
+        d1[n].PageDbEntryTyped? ::
+            d1[n].addrspace == d2[n].addrspace &&
+            d1[n].entry == d2[n].entry)
+}
+
+predicate enc_enc_integ_eq(s1:state, s2:state, d1:PageDb, d2:PageDb, 
+    atkr:PageNr)
+    requires SaneState(s1) && SaneState(s2)
+    requires validPageDb(d1) && validPageDb(d2)
+    requires pageDbCorresponds(s1.m, d1) && pageDbCorresponds(s2.m, d2)
+    requires valDispPage(d1, atkr)
+    requires valAddrPage(d1, d1[atkr].addrspace)
+    requires enc_enc_integ_eqpdb(d1, d2, atkr)
+{
+    var atkr_asp := d1[atkr].addrspace;
+    var l1p := d1[atkr_asp].entry.l1ptnr; // same in both d1, d2 because of eqdb
+    nonStoppedL1(d1, l1p) <==> nonStoppedL1(d2, l1p) &&
+    nonStoppedL1(d1, l1p) ==> (
+        var atkr_pgs := PagesInTable(mkAbsPTable(d1, l1p));
+        // The set of pages the attacker can modify is the same
+        (WritablePagesInTable(mkAbsPTable(d1, l1p)) == 
+            WritablePagesInTable(mkAbsPTable(d2, l1p))) &&
+        // The contents of pages the attacker cannot modify is the same
+        (forall a | a in TheValidAddresses() && a !in atkr_pgs::
+            s1.m.addresses[a] == s2.m.addresses[a])
+    )
 }
